type/global.v
@@ -1,214 +1,162 @@
-From SST Require Export src.unscoped src.expressions.
-Require Import List String.
-Open Scope string_scope.
+From mathcomp Require Import ssreflect.seq all_ssreflect.
+From Paco Require Import paco pacotac.
+From SST Require Export src.expressions src.header.
+Require Import List String Coq.Arith.PeanoNat Relations. 
+Import ListNotations. 
 
 Notation part := string (only parsing).
 Notation label := nat (only parsing).
 
-Section global.
-Inductive global  : Type :=
-  | g_var : ( fin ) -> global 
-  | g_end : global 
-  | g_send : ( part   ) -> ( part   ) -> ( list (prod (prod (label  ) (sort  )) (global  )) ) -> global 
-  | g_rec : ( global   ) -> global .
+Section gtt.
 
-Lemma congr_g_end  : g_end  = g_end  .
-Proof. congruence. Qed.
+(* global session trees *)
+CoInductive gtt: Type :=
+  | gtt_end    : gtt
+  | gtt_send   : part -> part -> list (option (sort*gtt)) -> gtt.
 
-Lemma congr_g_send  { s0 : part   } { s1 : part   } { s2 : list (prod (prod (label  ) (sort  )) (global  )) } { t0 : part   } { t1 : part   } { t2 : list (prod (prod (label  ) (sort  )) (global  )) } (H1 : s0 = t0) (H2 : s1 = t1) (H3 : s2 = t2) : g_send  s0 s1 s2 = g_send  t0 t1 t2 .
-Proof. congruence. Qed.
-
-Lemma congr_g_rec  { s0 : global   } { t0 : global   } (H1 : s0 = t0) : g_rec  s0 = g_rec  t0 .
-Proof. congruence. Qed.
-
-Definition upRen_global_global   (xi : ( fin ) -> fin) : ( fin ) -> fin :=
-  (up_ren) xi.
-
-Fixpoint ren_global   (xiglobal : ( fin ) -> fin) (s : global ) : global  :=
-    match s return global  with
-    | g_var  s => (g_var ) (xiglobal s)
-    | g_end   => g_end 
-    | g_send  s0 s1 s2 => g_send  ((fun x => x) s0) ((fun x => x) s1) ((list_map (prod_map (prod_map (fun x => x) (fun x => x)) (ren_global xiglobal))) s2)
-    | g_rec  s0 => g_rec  ((ren_global (upRen_global_global xiglobal)) s0)
-    end.
-
-Definition up_global_global   (sigma : ( fin ) -> global ) : ( fin ) -> global  :=
-  (scons) ((g_var ) (var_zero)) ((funcomp) (ren_global (shift)) sigma).
-
-Fixpoint subst_global   (sigmaglobal : ( fin ) -> global ) (s : global ) : global  :=
-    match s return global  with
-    | g_var  s => sigmaglobal s
-    | g_end   => g_end 
-    | g_send  s0 s1 s2 => g_send  ((fun x => x) s0) ((fun x => x) s1) ((list_map (prod_map (prod_map (fun x => x) (fun x => x)) (subst_global sigmaglobal))) s2)
-    | g_rec  s0 => g_rec  ((subst_global (up_global_global sigmaglobal)) s0)
-    end.
-
-Fixpoint unfold_grec (s: global): global :=
+Definition gtt_id (s: gtt): gtt :=
   match s with
-    | g_rec g      => subst_global ((g_rec g) .: g_var) g
-    | g_send p q l =>
-      let fix next l :=
-        match l with
-          | nil                          => nil
-          | pair (pair lbl srt) g1 :: xs => pair (pair lbl srt) (unfold_grec g1) :: next xs 
-        end 
-      in g_send p q (next l)
-    | _            => s
+    | gtt_end        => gtt_end
+    | gtt_send p q l => gtt_send p q l
   end.
 
-Let gt := g_rec (g_send "p" "q" (cons (pair (pair 0 sint) (g_var 0)) nil)).
-Print gt.
-Compute unfold_grec gt.
+Lemma gtt_eq: forall s, s = gtt_id s.
+Proof. intro s; destruct s; easy. Defined.
 
-Definition upId_global_global  (sigma : ( fin ) -> global ) (Eq : forall x, sigma x = (g_var ) x) : forall x, (up_global_global sigma) x = (g_var ) x :=
-  fun n => match n with
-  | S fin_n => (ap) (ren_global (shift)) (Eq fin_n)
-  | 0  => eq_refl
+
+Inductive global  : Type :=
+  | g_var : fin -> global 
+  | g_end : global 
+  | g_send : part -> part -> list (option (sort * global)) -> global 
+  | g_rec : global -> global.
+  
+Section global_ind_ref.
+  Variable P : global -> Prop.
+  Hypothesis P_var : forall n, P (g_var n).
+  Hypothesis P_end : P (g_end).
+  Hypothesis P_send : forall p q lis, List.Forall (fun u => u = None \/ (exists s g, u = Some (s, g) /\ P g)) lis -> P (g_send p q lis).
+  Hypothesis P_rec : forall g, P g -> P (g_rec g).
+  
+  Fixpoint global_ind_ref p : P p.
+  Proof.
+    destruct p.
+    - apply P_var.
+    - apply P_end.
+    - apply P_send.
+      induction l; try easy.
+      constructor; try easy.
+      destruct a. right. destruct p. exists s1. exists g. split; try easy.
+      left. easy.
+    - apply P_rec. easy.
+  Qed.
+End global_ind_ref.
+
+
+Fixpoint incr_freeG (fv m : fin) (G : global) := 
+  match G with 
+    | g_var n        => g_var (if fv <= n then (n + m) else n)
+    | g_end          => g_end 
+    | g_send p q lis => g_send p q (map (fun u => 
+          match u with 
+            | Some (s, g) => Some (s, incr_freeG fv m g)
+            | None        => None
+          end) lis)
+    | g_rec g        => g_rec (incr_freeG (S fv) m g)
   end.
 
-Fixpoint idSubst_global  (sigmaglobal : ( fin ) -> global ) (Eqglobal : forall x, sigmaglobal x = (g_var ) x) (s : global ) : subst_global sigmaglobal s = s :=
-    match s return subst_global sigmaglobal s = s with
-    | g_var  s => Eqglobal s
-    | g_end   => congr_g_end 
-    | g_send  s0 s1 s2 => congr_g_send ((fun x => (eq_refl) x) s0) ((fun x => (eq_refl) x) s1) ((list_id (prod_id (prod_id (fun x => (eq_refl) x) (fun x => (eq_refl) x)) (idSubst_global sigmaglobal Eqglobal))) s2)
-    | g_rec  s0 => congr_g_rec ((idSubst_global (up_global_global sigmaglobal) (upId_global_global (_) Eqglobal)) s0)
-    end.
+Inductive subst_global : fin -> fin -> global -> global -> global -> Prop := 
+  | subg_var_is   : forall G t m,                            subst_global t m G (g_var t) (incr_freeG 0 m G)
+  | subg_var_notz : forall G t m, t <> 0 ->                  subst_global t m G (g_var 0) (g_var 0)
+  | subg_var_not1 : forall G t t' m, t <> S t' -> t <= t' -> subst_global t m G (g_var (S t')) (g_var (t'))
+  | subg_var_not2 : forall G t t' m, t <> S t' -> t' < t  -> subst_global t m G (g_var (S t')) (g_var (S t'))
+  | subg_end      : forall G t m,                            subst_global t m G g_end g_end
+  | subg_send     : forall G t m p q xs ys, List.Forall2 (fun u v => 
+                           (u = None /\ v = None) \/
+                           (exists s g g', u = Some(s, g) /\ v = Some(s, g') /\ subst_global t m G g g')
+                                                  ) xs ys -> subst_global t m G (g_send p q xs) (g_send p q ys)
+  | subg_rec      : forall G t m P Q, subst_global (S t) (S m) G P Q -> subst_global t m G (g_rec P) (g_rec Q). 
 
-Definition upExtRen_global_global   (xi : ( fin ) -> fin) (zeta : ( fin ) -> fin) (Eq : forall x, xi x = zeta x) : forall x, (upRen_global_global xi) x = (upRen_global_global zeta) x :=
-  fun n => match n with
-  | S fin_n => (ap) (shift) (Eq fin_n)
-  | 0  => eq_refl
-  end.
 
-Fixpoint extRen_global   (xiglobal : ( fin ) -> fin) (zetaglobal : ( fin ) -> fin) (Eqglobal : forall x, xiglobal x = zetaglobal x) (s : global ) : ren_global xiglobal s = ren_global zetaglobal s :=
-    match s return ren_global xiglobal s = ren_global zetaglobal s with
-    | g_var  s => (ap) (g_var ) (Eqglobal s)
-    | g_end   => congr_g_end 
-    | g_send  s0 s1 s2 => congr_g_send ((fun x => (eq_refl) x) s0) ((fun x => (eq_refl) x) s1) ((list_ext (prod_ext (prod_ext (fun x => (eq_refl) x) (fun x => (eq_refl) x)) (extRen_global xiglobal zetaglobal Eqglobal))) s2)
-    | g_rec  s0 => congr_g_rec ((extRen_global (upRen_global_global xiglobal) (upRen_global_global zetaglobal) (upExtRen_global_global (_) (_) Eqglobal)) s0)
-    end.
+Inductive betaG : relation global := 
+  | lttS : forall G G', subst_global 0 0 (g_rec G) G G' -> betaG (g_rec G) G'.
 
-Definition upExt_global_global   (sigma : ( fin ) -> global ) (tau : ( fin ) -> global ) (Eq : forall x, sigma x = tau x) : forall x, (up_global_global sigma) x = (up_global_global tau) x :=
-  fun n => match n with
-  | S fin_n => (ap) (ren_global (shift)) (Eq fin_n)
-  | 0  => eq_refl
-  end.
+Inductive gttT (R : global -> gtt -> Prop) : global -> gtt -> Prop := 
+  | gttT_end  : gttT R g_end gtt_end
+  | gttT_send : forall p q xs ys, List.Forall2 (fun u v => (u = None /\ v = None) \/ (exists s g g', u = Some(s, g) /\ v = Some(s, g') /\ R g g')) xs ys -> gttT R (g_send p q xs) (gtt_send p q ys)
+  | gttT_rec  : forall G Q G', subst_global 0 0 (g_rec G) G Q -> R Q G' -> gttT R (g_rec G) G'.
 
-Fixpoint ext_global   (sigmaglobal : ( fin ) -> global ) (tauglobal : ( fin ) -> global ) (Eqglobal : forall x, sigmaglobal x = tauglobal x) (s : global ) : subst_global sigmaglobal s = subst_global tauglobal s :=
-    match s return subst_global sigmaglobal s = subst_global tauglobal s with
-    | g_var  s => Eqglobal s
-    | g_end   => congr_g_end 
-    | g_send  s0 s1 s2 => congr_g_send ((fun x => (eq_refl) x) s0) ((fun x => (eq_refl) x) s1) ((list_ext (prod_ext (prod_ext (fun x => (eq_refl) x) (fun x => (eq_refl) x)) (ext_global sigmaglobal tauglobal Eqglobal))) s2)
-    | g_rec  s0 => congr_g_rec ((ext_global (up_global_global sigmaglobal) (up_global_global tauglobal) (upExt_global_global (_) (_) Eqglobal)) s0)
-    end.
+Definition gttTC G G' := paco2 gttT bot2 G G'.
 
-Definition up_ren_ren_global_global    (xi : ( fin ) -> fin) (tau : ( fin ) -> fin) (theta : ( fin ) -> fin) (Eq : forall x, ((funcomp) tau xi) x = theta x) : forall x, ((funcomp) (upRen_global_global tau) (upRen_global_global xi)) x = (upRen_global_global theta) x :=
-  up_ren_ren xi tau theta Eq.
+Inductive wfG : global -> Prop := 
+  | wfg_var : forall n, wfG (g_var n)
+  | wfg_end : wfG g_end
+  | wfg_send : forall p q lis, SList lis -> p <> q -> List.Forall (fun u => u = None \/ (exists s g, u = Some(s, g) /\ wfG g)) lis -> wfG (g_send p q lis)
+  | wfg_rec : forall g, wfG g -> wfG (g_rec g).
 
-Fixpoint compRenRen_global    (xiglobal : ( fin ) -> fin) (zetaglobal : ( fin ) -> fin) (rhoglobal : ( fin ) -> fin) (Eqglobal : forall x, ((funcomp) zetaglobal xiglobal) x = rhoglobal x) (s : global ) : ren_global zetaglobal (ren_global xiglobal s) = ren_global rhoglobal s :=
-    match s return ren_global zetaglobal (ren_global xiglobal s) = ren_global rhoglobal s with
-    | g_var  s => (ap) (g_var ) (Eqglobal s)
-    | g_end   => congr_g_end 
-    | g_send  s0 s1 s2 => congr_g_send ((fun x => (eq_refl) x) s0) ((fun x => (eq_refl) x) s1) ((list_comp (prod_comp (prod_comp (fun x => (eq_refl) x) (fun x => (eq_refl) x)) (compRenRen_global xiglobal zetaglobal rhoglobal Eqglobal))) s2)
-    | g_rec  s0 => congr_g_rec ((compRenRen_global (upRen_global_global xiglobal) (upRen_global_global zetaglobal) (upRen_global_global rhoglobal) (up_ren_ren (_) (_) (_) Eqglobal)) s0)
-    end.
+Inductive guardG : fin -> fin -> global -> Prop :=  
+  | gg_nil : forall m G, guardG 0 m G
+  | gg_end : forall n m, guardG n m g_end
+  | gg_send : forall n m p q lis, List.Forall (fun u => u = None \/ (exists s g, u = Some(s, g) /\ guardG n m g)) lis -> guardG (S n) m (g_send p q lis)
+  | gg_rec : forall n m g Q, subst_global 0 0 (g_rec g) g Q -> guardG n m Q -> guardG n (S m) (g_rec g).
 
-Definition up_ren_subst_global_global    (xi : ( fin ) -> fin) (tau : ( fin ) -> global ) (theta : ( fin ) -> global ) (Eq : forall x, ((funcomp) tau xi) x = theta x) : forall x, ((funcomp) (up_global_global tau) (upRen_global_global xi)) x = (up_global_global theta) x :=
-  fun n => match n with
-  | S fin_n => (ap) (ren_global (shift)) (Eq fin_n)
-  | 0  => eq_refl
-  end.
 
-Fixpoint compRenSubst_global    (xiglobal : ( fin ) -> fin) (tauglobal : ( fin ) -> global ) (thetaglobal : ( fin ) -> global ) (Eqglobal : forall x, ((funcomp) tauglobal xiglobal) x = thetaglobal x) (s : global ) : subst_global tauglobal (ren_global xiglobal s) = subst_global thetaglobal s :=
-    match s return subst_global tauglobal (ren_global xiglobal s) = subst_global thetaglobal s with
-    | g_var  s => Eqglobal s
-    | g_end   => congr_g_end 
-    | g_send  s0 s1 s2 => congr_g_send ((fun x => (eq_refl) x) s0) ((fun x => (eq_refl) x) s1) ((list_comp (prod_comp (prod_comp (fun x => (eq_refl) x) (fun x => (eq_refl) x)) (compRenSubst_global xiglobal tauglobal thetaglobal Eqglobal))) s2)
-    | g_rec  s0 => congr_g_rec ((compRenSubst_global (upRen_global_global xiglobal) (up_global_global tauglobal) (up_global_global thetaglobal) (up_ren_subst_global_global (_) (_) (_) Eqglobal)) s0)
-    end.
 
-Definition up_subst_ren_global_global    (sigma : ( fin ) -> global ) (zetaglobal : ( fin ) -> fin) (theta : ( fin ) -> global ) (Eq : forall x, ((funcomp) (ren_global zetaglobal) sigma) x = theta x) : forall x, ((funcomp) (ren_global (upRen_global_global zetaglobal)) (up_global_global sigma)) x = (up_global_global theta) x :=
-  fun n => match n with
-  | S fin_n => (eq_trans) (compRenRen_global (shift) (upRen_global_global zetaglobal) ((funcomp) (shift) zetaglobal) (fun x => eq_refl) (sigma fin_n)) ((eq_trans) ((eq_sym) (compRenRen_global zetaglobal (shift) ((funcomp) (shift) zetaglobal) (fun x => eq_refl) (sigma fin_n))) ((ap) (ren_global (shift)) (Eq fin_n)))
-  | 0  => eq_refl
-  end.
+Lemma guardL_more : forall n m k G, guardG n m G -> m <= k -> guardG n k G.
+Proof.
+  induction n; intros; try easy.
+  - apply gg_nil.
+  - revert IHn H H0. revert n k G. induction m; intros; try easy.
+    inversion H. subst. 
+    - apply gg_end.
+    - subst. apply gg_send; try easy.
+      clear H. revert IHn H0 H2. revert n k p.
+      induction lis; intros; try easy.
+      inversion H2. subst. clear H2.
+      constructor.
+      - destruct H3. subst. left. easy.
+        right. destruct H. destruct H. destruct H. subst. exists x. exists x0.
+        split; try easy. apply IHn with (m := 0); try easy.
+      - apply IHlis; try easy.
+    - destruct G.
+      - inversion H.
+      - apply gg_end.
+      - apply gg_send.
+        inversion H. subst.
+        revert IHm IHn H H0 H4. revert m n k s.
+        induction l; intros; try easy.
+        inversion H4. subst.
+        constructor.
+        - destruct H3. subst. left. easy.
+          destruct H1. destruct H1. destruct H1. subst. right.
+          exists x. exists x0. split; try easy.
+          apply IHn with (m := m.+1); try easy.
+        - apply IHl with (m := m) (s := s); try easy.
+        apply gg_send. easy.
+      - inversion H. subst.
+        destruct k; try easy.
+        apply gg_rec with (Q := Q); try easy.
+        apply IHm; try easy.
+Qed.
 
-Fixpoint compSubstRen_global    (sigmaglobal : ( fin ) -> global ) (zetaglobal : ( fin ) -> fin) (thetaglobal : ( fin ) -> global ) (Eqglobal : forall x, ((funcomp) (ren_global zetaglobal) sigmaglobal) x = thetaglobal x) (s : global ) : ren_global zetaglobal (subst_global sigmaglobal s) = subst_global thetaglobal s :=
-    match s return ren_global zetaglobal (subst_global sigmaglobal s) = subst_global thetaglobal s with
-    | g_var  s => Eqglobal s
-    | g_end   => congr_g_end 
-    | g_send  s0 s1 s2 => congr_g_send ((fun x => (eq_refl) x) s0) ((fun x => (eq_refl) x) s1) ((list_comp (prod_comp (prod_comp (fun x => (eq_refl) x) (fun x => (eq_refl) x)) (compSubstRen_global sigmaglobal zetaglobal thetaglobal Eqglobal))) s2)
-    | g_rec  s0 => congr_g_rec ((compSubstRen_global (up_global_global sigmaglobal) (upRen_global_global zetaglobal) (up_global_global thetaglobal) (up_subst_ren_global_global (_) (_) (_) Eqglobal)) s0)
-    end.
+CoFixpoint Ga : gtt := gtt_send "Alice" "Bob" [Some (snat, Ga)].
 
-Definition up_subst_subst_global_global    (sigma : ( fin ) -> global ) (tauglobal : ( fin ) -> global ) (theta : ( fin ) -> global ) (Eq : forall x, ((funcomp) (subst_global tauglobal) sigma) x = theta x) : forall x, ((funcomp) (subst_global (up_global_global tauglobal)) (up_global_global sigma)) x = (up_global_global theta) x :=
-  fun n => match n with
-  | S fin_n => (eq_trans) (compRenSubst_global (shift) (up_global_global tauglobal) ((funcomp) (up_global_global tauglobal) (shift)) (fun x => eq_refl) (sigma fin_n)) ((eq_trans) ((eq_sym) (compSubstRen_global tauglobal (shift) ((funcomp) (ren_global (shift)) tauglobal) (fun x => eq_refl) (sigma fin_n))) ((ap) (ren_global (shift)) (Eq fin_n)))
-  | 0  => eq_refl
-  end.
+Example Grec : gttTC (g_rec (g_send "Alice" "Bob" [Some (snat, g_var 0)])) Ga.
+Proof.
+  pcofix CIH.
+  pfold. apply gttT_rec with (Q := g_send "Alice" "Bob" [(Some (snat, (g_rec (g_send "Alice" "Bob" [Some (snat, g_var 0)]))))]).
+  constructor. constructor. right.
+  exists snat. exists (g_var 0). exists (g_rec (g_send "Alice" "Bob" [Some (snat, g_var 0)])).
+  split; try easy. split; try easy. constructor. easy.
+  
+  rewrite (gtt_eq Ga). simpl.
+  left. pfold.
+  constructor. constructor. right. exists snat. exists (g_rec (g_send "Alice" "Bob" [Some (snat, g_var 0)])). exists Ga.
+  split; try easy. split; try easy.
+  right. easy. easy.
+Qed.
+  
 
-Fixpoint compSubstSubst_global    (sigmaglobal : ( fin ) -> global ) (tauglobal : ( fin ) -> global ) (thetaglobal : ( fin ) -> global ) (Eqglobal : forall x, ((funcomp) (subst_global tauglobal) sigmaglobal) x = thetaglobal x) (s : global ) : subst_global tauglobal (subst_global sigmaglobal s) = subst_global thetaglobal s :=
-    match s return subst_global tauglobal (subst_global sigmaglobal s) = subst_global thetaglobal s with
-    | g_var  s => Eqglobal s
-    | g_end   => congr_g_end 
-    | g_send  s0 s1 s2 => congr_g_send ((fun x => (eq_refl) x) s0) ((fun x => (eq_refl) x) s1) ((list_comp (prod_comp (prod_comp (fun x => (eq_refl) x) (fun x => (eq_refl) x)) (compSubstSubst_global sigmaglobal tauglobal thetaglobal Eqglobal))) s2)
-    | g_rec  s0 => congr_g_rec ((compSubstSubst_global (up_global_global sigmaglobal) (up_global_global tauglobal) (up_global_global thetaglobal) (up_subst_subst_global_global (_) (_) (_) Eqglobal)) s0)
-    end.
-
-Definition rinstInst_up_global_global   (xi : ( fin ) -> fin) (sigma : ( fin ) -> global ) (Eq : forall x, ((funcomp) (g_var ) xi) x = sigma x) : forall x, ((funcomp) (g_var ) (upRen_global_global xi)) x = (up_global_global sigma) x :=
-  fun n => match n with
-  | S fin_n => (ap) (ren_global (shift)) (Eq fin_n)
-  | 0  => eq_refl
-  end.
-
-Fixpoint rinst_inst_global   (xiglobal : ( fin ) -> fin) (sigmaglobal : ( fin ) -> global ) (Eqglobal : forall x, ((funcomp) (g_var ) xiglobal) x = sigmaglobal x) (s : global ) : ren_global xiglobal s = subst_global sigmaglobal s :=
-    match s return ren_global xiglobal s = subst_global sigmaglobal s with
-    | g_var  s => Eqglobal s
-    | g_end   => congr_g_end 
-    | g_send  s0 s1 s2 => congr_g_send ((fun x => (eq_refl) x) s0) ((fun x => (eq_refl) x) s1) ((list_ext (prod_ext (prod_ext (fun x => (eq_refl) x) (fun x => (eq_refl) x)) (rinst_inst_global xiglobal sigmaglobal Eqglobal))) s2)
-    | g_rec  s0 => congr_g_rec ((rinst_inst_global (upRen_global_global xiglobal) (up_global_global sigmaglobal) (rinstInst_up_global_global (_) (_) Eqglobal)) s0)
-    end.
-
-Lemma rinstInst_global   (xiglobal : ( fin ) -> fin) : ren_global xiglobal = subst_global ((funcomp) (g_var ) xiglobal) .
-Proof. exact ((FunctionalExtensionality.functional_extensionality _ _ ) (fun x => rinst_inst_global xiglobal (_) (fun n => eq_refl) x)). Qed.
-
-Lemma instId_global  : subst_global (g_var ) = id .
-Proof. exact ((FunctionalExtensionality.functional_extensionality _ _ ) (fun x => idSubst_global (g_var ) (fun n => eq_refl) ((id) x))). Qed.
-
-Lemma rinstId_global  : @ren_global   (id) = id .
-Proof. exact ((eq_trans) (rinstInst_global ((id) (_))) instId_global). Qed.
-
-Lemma varL_global   (sigmaglobal : ( fin ) -> global ) : (funcomp) (subst_global sigmaglobal) (g_var ) = sigmaglobal .
-Proof. exact ((FunctionalExtensionality.functional_extensionality _ _ ) (fun x => eq_refl)). Qed.
-
-Lemma varLRen_global   (xiglobal : ( fin ) -> fin) : (funcomp) (ren_global xiglobal) (g_var ) = (funcomp) (g_var ) xiglobal .
-Proof. exact ((FunctionalExtensionality.functional_extensionality _ _ ) (fun x => eq_refl)). Qed.
-
-Lemma compComp_global    (sigmaglobal : ( fin ) -> global ) (tauglobal : ( fin ) -> global ) (s : global ) : subst_global tauglobal (subst_global sigmaglobal s) = subst_global ((funcomp) (subst_global tauglobal) sigmaglobal) s .
-Proof. exact (compSubstSubst_global sigmaglobal tauglobal (_) (fun n => eq_refl) s). Qed.
-
-Lemma compComp'_global    (sigmaglobal : ( fin ) -> global ) (tauglobal : ( fin ) -> global ) : (funcomp) (subst_global tauglobal) (subst_global sigmaglobal) = subst_global ((funcomp) (subst_global tauglobal) sigmaglobal) .
-Proof. exact ((FunctionalExtensionality.functional_extensionality _ _ ) (fun n => compComp_global sigmaglobal tauglobal n)). Qed.
-
-Lemma compRen_global    (sigmaglobal : ( fin ) -> global ) (zetaglobal : ( fin ) -> fin) (s : global ) : ren_global zetaglobal (subst_global sigmaglobal s) = subst_global ((funcomp) (ren_global zetaglobal) sigmaglobal) s .
-Proof. exact (compSubstRen_global sigmaglobal zetaglobal (_) (fun n => eq_refl) s). Qed.
-
-Lemma compRen'_global    (sigmaglobal : ( fin ) -> global ) (zetaglobal : ( fin ) -> fin) : (funcomp) (ren_global zetaglobal) (subst_global sigmaglobal) = subst_global ((funcomp) (ren_global zetaglobal) sigmaglobal) .
-Proof. exact ((FunctionalExtensionality.functional_extensionality _ _ ) (fun n => compRen_global sigmaglobal zetaglobal n)). Qed.
-
-Lemma renComp_global    (xiglobal : ( fin ) -> fin) (tauglobal : ( fin ) -> global ) (s : global ) : subst_global tauglobal (ren_global xiglobal s) = subst_global ((funcomp) tauglobal xiglobal) s .
-Proof. exact (compRenSubst_global xiglobal tauglobal (_) (fun n => eq_refl) s). Qed.
-
-Lemma renComp'_global    (xiglobal : ( fin ) -> fin) (tauglobal : ( fin ) -> global ) : (funcomp) (subst_global tauglobal) (ren_global xiglobal) = subst_global ((funcomp) tauglobal xiglobal) .
-Proof. exact ((FunctionalExtensionality.functional_extensionality _ _ ) (fun n => renComp_global xiglobal tauglobal n)). Qed.
-
-Lemma renRen_global    (xiglobal : ( fin ) -> fin) (zetaglobal : ( fin ) -> fin) (s : global ) : ren_global zetaglobal (ren_global xiglobal s) = ren_global ((funcomp) zetaglobal xiglobal) s .
-Proof. exact (compRenRen_global xiglobal zetaglobal (_) (fun n => eq_refl) s). Qed.
-
-Lemma renRen'_global    (xiglobal : ( fin ) -> fin) (zetaglobal : ( fin ) -> fin) : (funcomp) (ren_global zetaglobal) (ren_global xiglobal) = ren_global ((funcomp) zetaglobal xiglobal) .
-Proof. exact ((FunctionalExtensionality.functional_extensionality _ _ ) (fun n => renRen_global xiglobal zetaglobal n)). Qed.
-
-End global.
+End gtt.
 
 
 
@@ -216,50 +164,3 @@ End global.
 
 
 
-
-
-Global Instance Subst_global   : Subst1 (( fin ) -> global ) (global ) (global ) := @subst_global   .
-
-Global Instance Ren_global   : Ren1 (( fin ) -> fin) (global ) (global ) := @ren_global   .
-
-Global Instance VarInstance_global  : Var (fin) (global ) := @g_var  .
-
-Notation "x '__global'" := (g_var x) (at level 5, format "x __global") : subst_scope.
-
-Notation "x '__global'" := (@ids (_) (_) VarInstance_global x) (at level 5, only printing, format "x __global") : subst_scope.
-
-Notation "'var'" := (g_var) (only printing, at level 1) : subst_scope.
-
-Class Up_global X Y := up_global : ( X ) -> Y.
-
-Notation "↑__global" := (up_global) (only printing) : subst_scope.
-
-Notation "↑__global" := (up_global_global) (only printing) : subst_scope.
-
-Global Instance Up_global_global   : Up_global (_) (_) := @up_global_global   .
-
-Notation "s [ sigmaglobal ]" := (subst_global sigmaglobal s) (at level 7, left associativity, only printing) : subst_scope.
-
-Notation "[ sigmaglobal ]" := (subst_global sigmaglobal) (at level 1, left associativity, only printing) : fscope.
-
-Notation "s ⟨ xiglobal ⟩" := (ren_global xiglobal s) (at level 7, left associativity, only printing) : subst_scope.
-
-Notation "⟨ xiglobal ⟩" := (ren_global xiglobal) (at level 1, left associativity, only printing) : fscope.
-
-Ltac auto_unfold := repeat unfold subst1,  subst2,  Subst1,  Subst2,  ids,  ren1,  ren2,  Ren1,  Ren2,  Subst_global,  Ren_global,  VarInstance_global.
-
-Tactic Notation "auto_unfold" "in" "*" := repeat unfold subst1,  subst2,  Subst1,  Subst2,  ids,  ren1,  ren2,  Ren1,  Ren2,  Subst_global,  Ren_global,  VarInstance_global in *.
-
-Ltac asimpl' := repeat first [progress rewrite ?instId_global| progress rewrite ?compComp_global| progress rewrite ?compComp'_global| progress rewrite ?rinstId_global| progress rewrite ?compRen_global| progress rewrite ?compRen'_global| progress rewrite ?renComp_global| progress rewrite ?renComp'_global| progress rewrite ?renRen_global| progress rewrite ?renRen'_global| progress rewrite ?varL_global| progress rewrite ?varLRen_global| progress (unfold up_ren, upRen_global_global, up_global_global)| progress (cbn [subst_global ren_global])| fsimpl].
-
-Ltac asimpl := repeat try unfold_funcomp; auto_unfold in *; asimpl'; repeat try unfold_funcomp.
-
-Tactic Notation "asimpl" "in" hyp(J) := revert J; asimpl; intros J.
-
-Tactic Notation "auto_case" := auto_case (asimpl; cbn; eauto).
-
-Tactic Notation "asimpl" "in" "*" := auto_unfold in *; repeat first [progress rewrite ?instId_global in *| progress rewrite ?compComp_global in *| progress rewrite ?compComp'_global in *| progress rewrite ?rinstId_global in *| progress rewrite ?compRen_global in *| progress rewrite ?compRen'_global in *| progress rewrite ?renComp_global in *| progress rewrite ?renComp'_global in *| progress rewrite ?renRen_global in *| progress rewrite ?renRen'_global in *| progress rewrite ?varL_global in *| progress rewrite ?varLRen_global in *| progress (unfold up_ren, upRen_global_global, up_global_global in *)| progress (cbn [subst_global ren_global] in *)| fsimpl in *].
-
-Ltac substify := auto_unfold; try repeat (erewrite rinstInst_global).
-
-Ltac renamify := auto_unfold; try repeat (erewrite <- rinstInst_global).
