process/inversion.v
@@ -1,109 +1,654 @@
-From SST Require Import src.unscoped src.expressions process.processes process.typecheck type.global tree.global tree.local.
+From SST Require Import src.expressions process.processes process.typecheck type.global type.local type.isomorphism.
+From mathcomp Require Import ssreflect.seq.
 Require Import List String Datatypes ZArith Relations PeanoNat.
 Open Scope list_scope.
-From mathcomp Require Import ssreflect.seq.
 Import ListNotations.
 From Paco Require Import paco.
 
-Lemma typable_implies_wfC_helper : forall Pr STT,
-  Forall2
-       (fun (u : option process) (v : option (sort * ltt)) =>
-        u = None /\ v = None \/
-        (exists (p : process) (s : sort) (t : ltt),
-           u = Some p /\ v = Some (s, t) /\ wfC t)) Pr STT ->
-  Forall
-  (fun u : option (sort * ltt) =>
-   u = None \/
-   (exists (s : sort) (t : ltt), u = Some (s, t) /\ upaco1 wf bot1 t))
-  STT.
+
+Lemma mon_lttT : monotone2 lttT.
 Proof.
-  intro Pr. induction Pr; intros; try easy.
-  destruct STT; try easy.
-  destruct STT; try easy.
-  specialize(Forall2_cons_iff (fun (u : option process) (v : option (sort * ltt)) =>
-       u = None /\ v = None \/
-       (exists (p : process) (s : sort) (t : ltt),
-          u = Some p /\ v = Some (s, t) /\ wfC t)) a o Pr STT); intros.
-  destruct H0. clear H1. specialize(H0 H); intros. clear H. destruct H0.
-  specialize(IHPr STT H0); intros.
-  apply Forall_cons; try easy.
-  destruct H; try easy. left; easy. right.
-  destruct H. destruct H. destruct H. exists x0, x1. destruct H. destruct H1. 
-  split. easy. unfold upaco1. left. easy.
+  unfold monotone2. intros. induction IN; intros; try easy.
+  - apply lttT_end.
+  - apply lttT_send; try easy.
+    - revert H LE. revert r r' p ys.
+      induction xs; intros; try easy.
+      destruct ys; try easy.
+      destruct ys; try easy.
+      inversion H. subst.
+      constructor.
+      - destruct H3. left. easy.
+        destruct H0. destruct H0. destruct H0. destruct H0. destruct H1. subst. right.
+        exists x. exists x0. exists x1. split; try easy. split; try easy.
+        apply LE; try easy.
+      - apply IHxs with (r := r); try easy.
+  - apply lttT_recv; try easy.
+    - revert H LE. revert r r' p ys.
+      induction xs; intros; try easy.
+      destruct ys; try easy.
+      destruct ys; try easy.
+      inversion H. subst.
+      constructor.
+      - destruct H3. left. easy.
+        destruct H0. destruct H0. destruct H0. destruct H0. destruct H1. subst. right.
+        exists x. exists x0. exists x1. split; try easy. split; try easy.
+        apply LE; try easy.
+      - apply IHxs with (r := r); try easy.
+  - apply lttT_rec with (Q := Q); try easy.
+
 Qed.
 
-Lemma extended_SList : forall l S T, SList (extendLTT l [] (Some (S, T))).
+Lemma triad_le :  forall m t',
+                  is_true (ssrnat.leq m t') ->
+                  is_true (ssrnat.leq (S t') m) -> False.
 Proof.
-  intro l. induction l; try easy.
+Admitted.
+  
+
+Lemma subst_injL : forall m n G G1 Q Q0, subst_local m n G G1 Q0 -> subst_local m n G G1 Q -> Q = Q0.
+Proof.
+  intros m n G G1.
+  revert m n G. induction G1 using local_ind_ref; intros; try easy.
+  inversion H. subst. 
+  - inversion H0; try easy. 
+  - subst. inversion H0; try easy.
+  - subst. inversion H0; try easy.
+    subst. specialize(triad_le m t' H6 H8); try easy.
+  - subst. inversion H0; try easy. 
+    subst. specialize(triad_le m t' H8 H6); try easy.
+  
+  inversion H. subst. inversion H0. subst. easy.
+  
+  inversion H0. subst. inversion H1. subst.
+  assert (ys0 = ys). {
+    clear H0 H1. revert H H8 H9. revert p m n G ys ys0.
+    induction lis; intros; try easy.
+    destruct ys; try easy. destruct ys0; try easy.
+    destruct ys; try easy. destruct ys0; try easy.
+    inversion H. subst. clear H.
+    inversion H8. subst. clear H8.
+    inversion H9. subst. clear H9.
+    specialize(IHlis p m n G ys ys0 H3 H6 H8). subst.
+    clear H3 H6 H8.
+    destruct H4. destruct H. subst.
+    destruct H5. destruct H. subst. easy.
+    destruct H. destruct H. destruct H. easy.
+    destruct H. destruct H. destruct H. destruct H. destruct H0. subst.
+    destruct H5; try easy.
+    destruct H. destruct H. destruct H. destruct H. destruct H0. 
+    inversion H. subst. 
+    destruct H2; try easy. destruct H0. destruct H0. destruct H0. 
+    inversion H0. subst.
+    specialize(H2 m n G x1 x4 H3 H1). subst. easy.
+  }
+  subst. easy.
+  
+  inversion H0. subst. inversion H1. subst.
+  assert (ys0 = ys). {
+    clear H0 H1. revert H H8 H9. revert p m n G ys ys0.
+    induction lis; intros; try easy.
+    destruct ys; try easy. destruct ys0; try easy.
+    destruct ys; try easy. destruct ys0; try easy.
+    inversion H. subst. clear H.
+    inversion H8. subst. clear H8.
+    inversion H9. subst. clear H9.
+    specialize(IHlis p m n G ys ys0 H3 H6 H8). subst.
+    clear H3 H6 H8.
+    destruct H4. destruct H. subst.
+    destruct H5. destruct H. subst. easy.
+    destruct H. destruct H. destruct H. easy.
+    destruct H. destruct H. destruct H. destruct H. destruct H0. subst.
+    destruct H5; try easy.
+    destruct H. destruct H. destruct H. destruct H. destruct H0. 
+    inversion H. subst. 
+    destruct H2; try easy. destruct H0. destruct H0. destruct H0. 
+    inversion H0. subst.
+    specialize(H2 m n G x1 x4 H3 H1). subst. easy.
+  }
+  subst. easy.
+  
+  inversion H. subst. inversion H0. subst.
+  specialize(IHG1 (S m) (S n) G Q1 Q0 H6 H5). subst. easy.
 Qed.
 
-Lemma typable_implies_wfC_helper2 : forall p l S T,
-  wfC T ->
-  wf (upaco1 wf bot1) (ltt_send p (extendLTT l [] (Some (S, T)))).
+Lemma wfL_after_incr : forall G1 m n,
+     wfL G1 -> wfL (incr_freeL m n G1).
 Proof.
-  intros p l. induction l; intros; try easy.
-  simpl in *.
-  apply wf_send; try easy. apply Forall_cons; try easy. right.
-  exists S, T. split. easy. unfold upaco1. unfold wfC in H. left. easy.
-  simpl. 
-  constructor. simpl. apply extended_SList.
-  apply Forall_cons; try easy. left. easy.
-  specialize(IHl S T H); intros. inversion IHl; try easy.
+  induction G1 using local_ind_ref; intros; try easy.
+  - simpl in *.
+    constructor.
+  - revert m n H0 H. revert p.
+    induction lis; intros; try easy.
+    - inversion H. subst. clear H.
+      inversion H0. subst. inversion H5. subst.
+      specialize(SList_f a lis H2); intros.
+      destruct H.
+      - assert (wfL (incr_freeL m n (l_send p lis))).
+        {
+          apply IHlis; try easy.
+          inversion H0. subst. inversion H5. subst.
+          constructor; try easy.
+        }
+        destruct H6. subst.
+        - constructor. 
+          {
+            simpl. clear IHlis H3 H0 H4 H5 H2 H7 H1. 
+            revert m n p H. induction lis; intros; try easy.
+            specialize(SList_f a lis H); intros.
+            destruct H0.
+            - apply SList_b. apply IHlis; try easy.
+            - destruct H0. destruct H1. subst. 
+            simpl. destruct x; try easy.
+          }
+          constructor; try easy. left. easy.
+          {
+            clear IHlis H3 H0 H5 H2 H H1. clear p.
+            revert H4. revert m n. induction lis; intros; try easy. 
+            inversion H4. inversion H7. subst. clear H4 H7.
+            constructor. 
+            - destruct H1. subst. left. easy.
+            - destruct H. destruct H. destruct H. subst. right.
+              exists x. exists (incr_freeL m n x0). split; try easy. apply H0.
+              destruct H6; try easy. destruct H. destruct H. destruct H. inversion H. subst. easy.
+            - apply IHlis; try easy.
+          }
+        - destruct H6. destruct H6. destruct H6. subst. 
+          constructor; try easy.
+          {
+             apply SList_b.
+             clear IHlis H3 H0 H4 H5 H2 H8 H7 H1. clear x x0 p.
+             revert m n H.
+             induction lis; intros; try easy.
+             specialize(SList_f a lis H); intros.
+             destruct H0. apply SList_b. apply IHlis; try easy.
+             destruct H0. destruct H1. subst. destruct x. easy.
+          }
+          constructor. right. exists x. exists (incr_freeL m n x0).
+          split; try easy.
+          destruct H3; try easy. destruct H3. destruct H3. destruct H3. inversion H3. subst. 
+          apply H6; try easy.
+          {
+            clear IHlis H3 H0 H5 H2 H H1. clear p.
+            revert H4. revert m n. induction lis; intros; try easy. 
+            inversion H4. inversion H7. subst. clear H4 H7.
+            constructor. 
+            - destruct H1. subst. left. easy.
+            - destruct H. destruct H. destruct H. subst. right.
+              exists x1. exists (incr_freeL m n x2). split; try easy. apply H0.
+              destruct H6; try easy. destruct H. destruct H. destruct H. inversion H. subst. easy.
+            - apply IHlis; try easy.
+          }
+        - destruct H. destruct H1. subst.
+          destruct H6; try easy. destruct H. destruct H. destruct H. subst.
+          destruct H3; try easy. destruct H3. destruct H3. destruct H3. 
+          replace (Some x) with (Some (x2, x3)) in *. inversion H. subst. clear H H3 H4 H7 H5.
+          constructor; try easy. constructor; try easy.
+          right. exists x0. exists (incr_freeL m n x1).
+          split; try easy. apply H6; try easy.
+  - revert m n H0 H. revert p.
+    induction lis; intros; try easy.
+    - inversion H. subst. clear H.
+      inversion H0. subst. inversion H5. subst.
+      specialize(SList_f a lis H2); intros.
+      destruct H.
+      - assert (wfL (incr_freeL m n (l_recv p lis))).
+        {
+          apply IHlis; try easy.
+          inversion H0. subst. inversion H5. subst.
+          constructor; try easy.
+        }
+        destruct H6. subst.
+        - constructor. 
+          {
+            simpl. clear IHlis H3 H0 H4 H5 H2 H7 H1. 
+            revert m n p H. induction lis; intros; try easy.
+            specialize(SList_f a lis H); intros.
+            destruct H0.
+            - apply SList_b. apply IHlis; try easy.
+            - destruct H0. destruct H1. subst. 
+            simpl. destruct x; try easy.
+          }
+          constructor; try easy. left. easy.
+          {
+            clear IHlis H3 H0 H5 H2 H H1. clear p.
+            revert H4. revert m n. induction lis; intros; try easy. 
+            inversion H4. inversion H7. subst. clear H4 H7.
+            constructor. 
+            - destruct H1. subst. left. easy.
+            - destruct H. destruct H. destruct H. subst. right.
+              exists x. exists (incr_freeL m n x0). split; try easy. apply H0.
+              destruct H6; try easy. destruct H. destruct H. destruct H. inversion H. subst. easy.
+            - apply IHlis; try easy.
+          }
+        - destruct H6. destruct H6. destruct H6. subst. 
+          constructor; try easy.
+          {
+             apply SList_b.
+             clear IHlis H3 H0 H4 H5 H2 H8 H7 H1. clear x x0 p.
+             revert m n H.
+             induction lis; intros; try easy.
+             specialize(SList_f a lis H); intros.
+             destruct H0. apply SList_b. apply IHlis; try easy.
+             destruct H0. destruct H1. subst. destruct x. easy.
+          }
+          constructor. right. exists x. exists (incr_freeL m n x0).
+          split; try easy.
+          destruct H3; try easy. destruct H3. destruct H3. destruct H3. inversion H3. subst. 
+          apply H6; try easy.
+          {
+            clear IHlis H3 H0 H5 H2 H H1. clear p.
+            revert H4. revert m n. induction lis; intros; try easy. 
+            inversion H4. inversion H7. subst. clear H4 H7.
+            constructor. 
+            - destruct H1. subst. left. easy.
+            - destruct H. destruct H. destruct H. subst. right.
+              exists x1. exists (incr_freeL m n x2). split; try easy. apply H0.
+              destruct H6; try easy. destruct H. destruct H. destruct H. inversion H. subst. easy.
+            - apply IHlis; try easy.
+          }
+        - destruct H. destruct H1. subst.
+          destruct H6; try easy. destruct H. destruct H. destruct H. subst.
+          destruct H3; try easy. destruct H3. destruct H3. destruct H3. 
+          replace (Some x) with (Some (x2, x3)) in *. inversion H. subst. clear H H3 H4 H7 H5.
+          constructor; try easy. constructor; try easy.
+          right. exists x0. exists (incr_freeL m n x1).
+          split; try easy. apply H6; try easy.
+  - inversion H. subst.
+    constructor; try easy. apply IHG1; try easy.
+Qed.
+        
+  
+Lemma wfL_after_subst : forall Q G1 G2 m n,
+    wfL G1 -> wfL G2 -> subst_local m n G1 G2 Q -> wfL Q.
+Proof.
+  induction Q using local_ind_ref; intros; try easy.
+  - apply wfl_var.
+  - apply wfl_end.
+  - inversion H2; try easy. 
+    - subst.
+      apply wfL_after_incr. easy.
+    - subst.
+      inversion H1. subst.
+      revert H H0 H1 H2 H8 H5 H6.
+      revert p G1 m n xs.
+      induction lis; intros; try easy. 
+      - destruct xs; try easy.
+      - destruct xs; try easy.
+        specialize(SList_f o xs H5); intros. clear H5.
+        inversion H8. subst. clear H8. inversion H6. subst. clear H6.
+        destruct H3.
+        - constructor; try easy. apply SList_b.
+          {
+            clear IHlis H H0 H1 H2 H9 H7 H8. revert H11 H3. revert xs.
+            induction lis; intros; try easy.
+            destruct xs; try easy.
+            inversion H11. subst.
+            specialize(SList_f x l H3); intros. destruct H. 
+            - apply SList_b. apply IHlis with (xs := l); try easy.
+            - destruct H. destruct H0. subst. destruct lis; try easy.
+              destruct H2; try easy. destruct H. destruct H. destruct H. destruct H. destruct H0. subst. easy.
+          } 
+        - inversion H. subst. clear H.
+          assert (wfL (l_send p lis)). 
+          {
+            apply IHlis with (G1 := G1) (m := m) (n := n) (xs := xs); try easy.
+            inversion H1. subst. inversion H12. subst. clear H12.
+            constructor; try easy.
+            inversion H2. subst. inversion H13. subst. clear H13.
+            constructor; try easy.
+          }
+          inversion H. subst. constructor; try easy.
+          clear H11 H8 H10 H12 H13 IHlis.
+          destruct H6.
+          - left. easy.
+          - right. destruct H4. destruct H4. destruct H4. subst.
+            destruct H9; try easy. destruct H4. destruct H4. destruct H4. destruct H4. destruct H6. inversion H6. subst.
+            exists x1. exists x3. split; try easy.
+            destruct H7; try easy. destruct H4. destruct H4. destruct H4. inversion H4. subst. 
+            specialize(H5 G1 x0 m n). apply H5; try easy.
+        - destruct H3. destruct H4. subst.
+          destruct H9; try easy. destruct H3. destruct H3. destruct H3. destruct H3. destruct H4. inversion H3. subst.
+          destruct H7; try easy. destruct H4. destruct H4. destruct H4. inversion H4. subst. 
+          destruct lis; try easy.
+          constructor; try easy. constructor; try easy. right.
+          exists x. exists x2. split; try easy.
+          inversion H. subst. clear H. destruct H10; try easy. destruct H. destruct H. destruct H. inversion H. subst.
+          specialize(H7 G1 x3 m n). apply H7; try easy.
+  - inversion H2; try easy. 
+    - subst.
+      apply wfL_after_incr. easy.
+    - subst.
+      inversion H1. subst.
+      revert H H0 H1 H2 H8 H5 H6.
+      revert p G1 m n xs.
+      induction lis; intros; try easy. 
+      - destruct xs; try easy.
+      - destruct xs; try easy.
+        specialize(SList_f o xs H5); intros. clear H5.
+        inversion H8. subst. clear H8. inversion H6. subst. clear H6.
+        destruct H3.
+        - constructor; try easy. apply SList_b.
+          {
+            clear IHlis H H0 H1 H2 H9 H7 H8. revert H11 H3. revert xs.
+            induction lis; intros; try easy.
+            destruct xs; try easy.
+            inversion H11. subst.
+            specialize(SList_f x l H3); intros. destruct H. 
+            - apply SList_b. apply IHlis with (xs := l); try easy.
+            - destruct H. destruct H0. subst. destruct lis; try easy.
+              destruct H2; try easy. destruct H. destruct H. destruct H. destruct H. destruct H0. subst. easy.
+          } 
+        - inversion H. subst. clear H.
+          assert (wfL (l_recv p lis)). 
+          {
+            apply IHlis with (G1 := G1) (m := m) (n := n) (xs := xs); try easy.
+            inversion H1. subst. inversion H12. subst. clear H12.
+            constructor; try easy.
+            inversion H2. subst. inversion H13. subst. clear H13.
+            constructor; try easy.
+          }
+          inversion H. subst. constructor; try easy.
+          clear H11 H8 H10 H12 H13 IHlis.
+          destruct H6.
+          - left. easy.
+          - right. destruct H4. destruct H4. destruct H4. subst.
+            destruct H9; try easy. destruct H4. destruct H4. destruct H4. destruct H4. destruct H6. inversion H6. subst.
+            exists x1. exists x3. split; try easy.
+            destruct H7; try easy. destruct H4. destruct H4. destruct H4. inversion H4. subst. 
+            specialize(H5 G1 x0 m n). apply H5; try easy.
+        - destruct H3. destruct H4. subst.
+          destruct H9; try easy. destruct H3. destruct H3. destruct H3. destruct H3. destruct H4. inversion H3. subst.
+          destruct H7; try easy. destruct H4. destruct H4. destruct H4. inversion H4. subst. 
+          destruct lis; try easy.
+          constructor; try easy. constructor; try easy. right.
+          exists x. exists x2. split; try easy.
+          inversion H. subst. clear H. destruct H10; try easy. destruct H. destruct H. destruct H. inversion H. subst.
+          specialize(H7 G1 x3 m n). apply H7; try easy.
+  - inversion H1. subst.
+    apply wfL_after_incr; try easy.
+    subst.
+    specialize(IHQ G1 P (S m) (S n)). 
+    constructor. apply IHQ; try easy.
+    inversion H0. easy.
+Qed.
+  
+Lemma guard_break : forall x, (forall n, exists m, guardL n m (l_rec x)) -> exists T, multiS betaL (l_rec x) T /\  (forall n, exists m, guardL n m T) /\ (T = l_end \/ (exists p lis, T = l_send p lis \/ T = l_recv p lis)).
+Proof.
+  intros.
+  pose proof H as H1.
+  specialize(H1 1). destruct H1.
+  assert (exists T, multiS betaL (l_rec x) T /\
+  (T = l_end \/
+   (exists
+      (p : string) (lis : seq.seq (option (sort * local))),
+      T = l_send p lis \/ T = l_recv p lis))).
+  {
+    clear H. revert H0. revert x. induction x0; intros; try easy.
+    inversion H0. subst.
+    destruct Q; try easy.
+    - exists l_end.
+      split. apply multi_sing. constructor; try easy.
+      left. easy.
+    - exists (l_send s l).
+      split. apply multi_sing. constructor; try easy.
+      right. exists s. exists l. left. easy.
+    - exists (l_recv s l).
+      split. apply multi_sing. constructor; try easy.
+      right. exists s. exists l. right. easy.
+    - specialize(IHx0 Q H4). 
+      destruct IHx0. destruct H. exists x1. split; try easy.
+      apply multi_step with (y := (l_rec Q)).
+      constructor; try easy.
+      easy.
+  }
+  destruct H1. destruct H1. exists x1.
+  split; try easy. split; try easy.
+  clear H0 H2. clear x0.
+  revert H. induction H1; intros; try easy.
+  - inversion H. subst.
+    specialize(H0 n). destruct H0. 
+    inversion H0. subst.
+    - exists 0. apply gl_nil.
+    - subst. exists m.
+      specialize(subst_injL 0 0 (l_rec G) G y Q H3 H1); intros. subst. easy.
+  - inversion H. subst.
+    apply IHmultiS; try easy.
+    intros. specialize(H0 n0). destruct H0.
+    inversion H0. subst. exists 0. apply gl_nil.
+    subst. exists m.
+    specialize(subst_injL 0 0 (l_rec G) G y Q H4 H2); intros. subst. easy.
 Qed.
 
-Lemma SList_induc {A} : forall x (xs : list (option A)), SList (x :: xs) -> (xs = [] \/ SList xs).
+Lemma typable_implies_wfC_helper_p2 : forall x T',
+      lttTC (l_rec x) T' ->
+      wfL (l_rec x) -> 
+      (forall n, exists m, guardL n m (l_rec x)) ->
+      exists T, lttTC T T' /\ wfL T /\ (forall n, exists m, guardL n m T) /\ (T = l_end \/ (exists p lis, T = l_send p lis \/ T = l_recv p lis)).
 Proof.
-  intros. destruct xs.
-  left. easy. right. simpl in *. 
-  destruct o. destruct x. easy. easy. 
-  destruct x. easy. easy.
+      intros.
+      specialize(guard_break x H1); intros.
+      destruct H2. exists x0. destruct H2.
+      split.
+      - clear H0 H1 H3.
+        revert H. revert T'. induction H2; intros; try easy.
+        inversion H. subst. 
+        pinversion H0. subst. 
+        specialize(subst_injL 0 0 (l_rec G) G Q y H1 H3); intros. subst.
+        unfold lttTC. pfold. easy.
+        apply mon_lttT.
+      - apply IHmultiS; try easy.
+        inversion H. subst.
+        pinversion H0. subst. 
+        specialize(subst_injL 0 0 (l_rec G) G Q y H1 H4); intros. subst.
+        unfold lttTC. pfold. easy.
+        apply mon_lttT.
+      split; try easy.
+      - clear H H1 H3.
+        revert H0. revert T'. induction H2; intros; try easy.
+        inversion H. subst.
+        inversion H0. subst.
+        specialize(wfL_after_subst y (l_rec G) G 0 0); intros. apply H2; try easy.
+      - apply IHmultiS; try easy.
+         inversion H. subst.
+        inversion H0. subst.
+        specialize(wfL_after_subst y (l_rec G) G 0 0); intros. apply H3; try easy.
 Qed.
 
-Lemma SList_inducb {A} : forall x (xs : list (option A)), SList xs -> SList (x::xs).
+Lemma typable_implies_wfC_helper_recv : forall x p STT,
+      lttTC x (ltt_recv p STT) ->
+      wfL x -> 
+      (forall n, exists m, guardL n m x) ->
+      exists T, lttTC (l_recv p T) (ltt_recv p STT) /\ wfL (l_recv p T) /\ (forall n, exists m, guardL n m (l_recv p T)).
 Proof.
-  intros. simpl.
-  destruct x; try easy.
-  destruct xs; try easy.
+  induction x using local_ind_ref; intros; try easy.
+  - pinversion H.
+    apply mon_lttT.
+  - pinversion H.
+    apply mon_lttT.
+  - exists lis. 
+    pinversion H0. subst. 
+    apply mon_lttT.
+  - exists lis.
+    pinversion H0. subst.
+    split.
+    pfold. easy. easy.
+    apply mon_lttT.
+  - pinversion H. subst.
+    
+    specialize(typable_implies_wfC_helper_p2 x (ltt_recv p STT)); intros.
+    unfold lttTC in H2 at 1. 
+    assert (exists T : local,
+       lttTC T (ltt_recv p STT) /\
+       wfL T /\
+       (forall n : fin, exists m : fin, guardL n m T) /\
+       (T = l_end \/
+        (exists
+           (p : string) (lis : seq.seq (option (sort * local))),
+           T = l_send p lis \/ T = l_recv p lis))).
+    {
+      apply H2; try easy.
+      pfold. easy.
+    }
+    clear H2. destruct H5. destruct H2. destruct H5. destruct H6.
+    pinversion H2. subst.
+    - destruct H7; try easy. destruct H7. destruct H7. destruct H7. easy.
+      inversion H7. subst. exists x1. unfold lttTC. split. pfold. easy. easy.
+    - subst. destruct H7; try easy. destruct H7. destruct H7. destruct H7; try easy.
+    apply mon_lttT.
+    apply mon_lttT.
 Qed.
 
-Lemma typable_implies_wfC_helper3 : forall Pr STT,
+
+Lemma typable_implies_wfC_helper_recv2 : forall STT Pr p,
     SList Pr ->
     Forall2
        (fun (u : option process) (v : option (sort * ltt)) =>
         u = None /\ v = None \/
-        (exists (p : process) (s : sort) (t : ltt),
-           u = Some p /\ v = Some (s, t) /\ wfC t)) Pr STT ->
-    SList STT.
+        (exists (p : process) (s : sort) (t : ltt), u = Some p /\ v = Some (s, t) /\ wfC t)) Pr STT ->
+    wfC (ltt_recv p STT).
 Proof.
-  intro Pr. induction Pr; intros; try easy.
-  destruct STT; try easy.
-  specialize(Forall2_cons_iff (fun (u : option process) (v : option (sort * ltt)) =>
-        u = None /\ v = None \/
-        (exists (p : process) (s : sort) (t : ltt),
-           u = Some p /\ v = Some (s, t) /\ wfC t)) a o Pr STT); intros.
-  destruct H1. specialize(H1 H0). clear H0 H2.
-  destruct H1. destruct H0.
-  destruct H0. subst. simpl. apply IHPr; try easy.
-  destruct H0. destruct H0. destruct H0. destruct H0. destruct H2. subst.
-  
-  destruct Pr; try easy.
-  specialize(Forall2_length H1); intros. simpl in H0.
-  specialize(length_zero_iff_nil STT); intros. destruct H2. clear H4.
-  specialize(H2 (ssrfun.esym H0)). subst. easy.
-  apply SList_inducb. apply IHPr; try easy.
+  induction STT; intros; try easy.
+  - destruct Pr; try easy.
+  - destruct Pr; try easy.
+    inversion H0. subst.
+    unfold wfC. destruct H4.
+    - destruct H1. subst. 
+      specialize(IHSTT Pr p H H6).
+      unfold wfC in IHSTT. destruct IHSTT. destruct H1. destruct H2.
+      specialize(typable_implies_wfC_helper_recv x p STT H1 H2 H3); intros.
+      destruct H4. destruct H4. destruct H5. 
+      exists (l_recv p (None :: x0)).
+      split.
+      - pinversion H4. subst.
+        unfold lttTC. pfold. constructor. constructor; try easy. left. easy.
+        apply mon_lttT.
+      split; try easy.
+      - inversion H5. subst. constructor; try easy. constructor; try easy.
+        left. easy. 
+        intros. specialize(H7 n). destruct H7. inversion H7. subst. exists 0. apply gl_nil.
+        subst. exists x1. constructor; try easy. constructor; try easy. left. easy.
+    - destruct H1. destruct H1. destruct H1. destruct H1. destruct H2. subst. clear H0.
+      unfold wfC in H3. destruct H3. destruct H0. destruct H1.
+      specialize(SList_f (Some x) Pr H); intros. destruct H3.
+      - specialize(IHSTT Pr p H3 H6). 
+        unfold wfC in IHSTT. destruct IHSTT. destruct H4. destruct H5.
+        specialize(typable_implies_wfC_helper_recv x3 p STT H4 H5 H7); intros.
+        destruct H8. destruct H8. destruct H9.
+        exists (l_recv p (Some (x0, x2) :: x4)).
+        split.
+        - pfold. constructor.
+          pinversion H8. subst. constructor; try easy.
+          right. exists x0. exists x2. exists x1. split. easy. split. easy.
+          left. easy.
+          apply mon_lttT.
+        split.
+        - constructor; try easy.
+          specialize(SList_f (Some x) Pr H); intros.
+          {
+            clear H4 H5 H7 H H0 H1 H2 H3 H9 H10.
+            destruct H11.
+            apply SList_b. pinversion H8. subst. clear H8. clear p x3 x x0 x1 x2. 
+            revert H6 H1 H. revert Pr x4. induction STT; intros; try easy.
+            - destruct Pr; try easy.
+            - destruct Pr; try easy.
+              destruct x4; try easy.
+              inversion H6. subst. clear H6. inversion H1. subst. clear H1.
+              specialize(SList_f o Pr H); intros. destruct H0.
+              - apply SList_b. apply IHSTT with (Pr := Pr); try easy.
+              - destruct H0. destruct H1. subst.
+                destruct STT; try easy. destruct x4; try easy.
+                destruct H4; try easy. destruct H0. destruct H0. destruct H0. destruct H0. destruct H1. inversion H0. subst.
+                destruct H5; try easy. destruct H1. destruct H1. destruct H1. destruct H1. destruct H3. inversion H3. subst. easy.
+                apply mon_lttT.
+            - destruct H. subst. destruct STT; try easy.
+              pinversion H8. subst. destruct x4; try easy.
+              apply mon_lttT.
+          }
+        - pinversion H8. subst. constructor.
+          right. exists x0. exists x2. split; try easy.
+          inversion H9. subst. easy.
+          apply mon_lttT.
+        - clear H4 H5 H7 H H0 H1 H6 H3 H8 H9.
+          clear STT x3 Pr x x1.
+          intros.
+          destruct n. exists 0. apply gl_nil.
+          specialize(H2 n). specialize(H10 (S n)). destruct H2. destruct H10.
+          exists (ssrnat.maxn x1 x). apply gl_recv.
+          constructor.
+          - right. exists x0. exists x2. split; try easy.
+            specialize(guardL_more n x); intros. apply H1; try easy.
+            specialize(ssrnat.leq_maxr x1 x); intros. easy.
+          - inversion H0. subst. clear H0 H. clear p x0 x2. revert H4. revert n x x1.
+            induction x4; intros; try easy.
+            inversion H4. subst.
+            constructor; try easy.
+            destruct H1.
+            - left. easy.
+            - right. destruct H. destruct H. destruct H. subst. exists x0. exists x2.
+              split; try easy.
+              specialize(guardL_more n x1 (ssrnat.maxn x1 x) x2 H0); intros.
+              apply H.
+              specialize(ssrnat.leq_maxl x1 x); intros. easy.
+            apply IHx4; try easy.
+      - destruct H3. destruct H4. subst.
+        destruct STT; try easy. inversion H4. subst.
+        exists (l_recv p [Some (x0, x2)]).
+        split.
+        - unfold lttTC. pfold. constructor.
+          constructor. right. exists x0. exists x2. exists x1.
+          split. easy. split. easy.
+          left. easy.
+        - easy.
+        split.
+        - constructor. easy.
+          constructor. right. exists x0. exists x2. split; try easy.
+        - easy.
+        - intro. 
+          destruct n. exists 0. apply gl_nil.
+          specialize(H2 n). destruct H2.
+          exists x. apply gl_recv. constructor; try easy.
+          right. exists x0. exists x2. split. easy. easy.
 Qed.
   
-
 Lemma typable_implies_wfC [P : process] [Gs : ctxS] [Gt : ctxT] [T : ltt] :
   typ_proc Gs Gt P T -> wfC T.
 Proof.
   intros. induction H using typ_proc_ind_ref; try easy.
-  - unfold wfC. pfold. constructor.
-  - unfold wfC. pfold. constructor; try easy.
-    apply typable_implies_wfC_helper3 with (Pr := Pr); try easy.
-    apply typable_implies_wfC_helper with (Pr := Pr); try easy.
-  - unfold wfC. pfold. 
-    apply typable_implies_wfC_helper2; try easy.
+  - unfold wfC. exists l_end. split. pfold. constructor. 
+    split. apply wfl_end.
+    intros. exists 0. apply gl_end.
+  - apply typable_implies_wfC_helper_recv2 with (Pr := Pr); try easy.
+  - unfold wfC.
+    inversion IHtyp_proc. 
+    destruct H0. destruct H1.
+    exists (l_send p (extendLis l (Some (S, x)))).
+    unfold wfC in IHtyp_proc. destruct IHtyp_proc. destruct H3. destruct H4.
+    split.
+    - unfold lttTC. pfold. constructor.
+      induction l; intros; try easy.
+      simpl in *.
+      - constructor; try easy.
+        right. exists S. exists x. exists T. split. easy. split. easy.
+        unfold lttTC in H0. left. easy.
+      - simpl. constructor; try easy.
+        left. easy.
+    split.
+    - induction l; intros; try easy.
+      simpl in *.
+      - constructor; try easy.
+      - constructor; try easy. right. exists S. exists x. split; try easy.
+      - inversion IHl. subst.
+        constructor; try easy.
+        constructor; try easy. left. easy.
+      - intros.
+        destruct n; try easy.
+        - exists 0. apply gl_nil.
+        - specialize(H2 n). destruct H2.
+          exists x1. apply gl_send; try easy.
+          induction l; intros; try easy.
+          - simpl in *. constructor; try easy.
+            right. exists S. exists x. split; try easy.
+          - simpl. constructor; try easy. left. easy.
 Qed.
 
 Lemma _a23_a: forall p Q P Gs Gt T, 
@@ -151,12 +696,12 @@ Qed.
  *)
 Lemma _a23_bf: forall p l e Q P Gs Gt T, 
   typ_proc Gs Gt P T ->
-  P = (p_send p l e Q) -> exists S T', typ_expr Gs e S /\ typ_proc Gs Gt Q T' /\  subtypeC (ltt_send p (extendLTT l [] (Some (S,T')))) T.
+  P = (p_send p l e Q) -> exists S T', typ_expr Gs e S /\ typ_proc Gs Gt Q T' /\  subtypeC (ltt_send p (extendLis l (Some (S,T')))) T.
 Proof.
   intros. revert H0. induction H; intros; try easy.
   specialize(IHtyp_proc H2); intros. destruct IHtyp_proc. destruct H3. destruct H3. destruct H4.
   exists x. exists x0. split; try easy. split; try easy.
-  specialize(stTrans (ltt_send p (extendLTT l [] (Some (x, x0)))) t t' H5 H0); intros; try easy.
+  specialize(stTrans (ltt_send p (extendLis l (Some (x, x0)))) t t' H5 H0); intros; try easy.
   inversion H1. subst.
   exists S. exists T. split; try easy. split; try easy. apply stRefl. 
 Qed.
