process/subject_reduction.v
@@ -1,14 +1,14 @@
-From SST Require Export src.unscoped src.expressions process.processes process.typecheck type.global type.local tree.global tree.local process.beta process.sessions process.inversion.
+From SST Require Export src.expressions process.processes process.typecheck type.global type.local process.beta process.sessions process.inversion  type.isomorphism type.projection.
 Require Import List String Datatypes ZArith Relations PeanoNat.
 Open Scope list_scope.
 From Paco Require Import paco pacotac.
 Require Import Setoid Morphisms Coq.Program.Basics.
 Require Import Coq.Init.Datatypes.
 
+
 Inductive multiC : relation gtt := 
   | multiC_refl : forall G, multiC G G
   | multiC_step : forall G1 G2 G3 p q n, gttstepC G1 G2 p q n -> multiC G2 G3 -> multiC G1 G3.
-
 
 Lemma projection_cont_p : forall G x6 p q l x,
     gttstepC G x6 q p l -> projectionC G p (ltt_recv q x) -> exists T, projectionC x6 p T.
@@ -57,7 +57,7 @@ Admitted.
 
 Lemma _3_19_h : forall p q l G L1 L2 S T xs y,
   projectionC G p (ltt_send q L1) -> 
-  subtypeC (ltt_send q (extendLTT l nil (Datatypes.Some(S,T)))) (ltt_send q L1) ->
+  subtypeC (ltt_send q (extendLis l (Datatypes.Some(S,T)))) (ltt_send q L1) ->
   projectionC G q (ltt_recv p L2) -> 
   onth l xs = Some y ->
   subtypeC (ltt_recv p xs) (ltt_recv p L2) -> 
@@ -72,7 +72,7 @@ Admitted.
 
 Lemma _3_19_1 : forall p q l G G' L1 L2 S T,
   projectionC G p (ltt_send q L1) ->
-  subtypeC (ltt_send q (extendLTT l nil (Datatypes.Some (S,T)))) (ltt_send q L1) ->
+  subtypeC (ltt_send q (extendLis l (Datatypes.Some (S,T)))) (ltt_send q L1) ->
   gttstepC G G' p q l ->
   projectionC G' p L2 ->
   subtypeC T L2.
@@ -197,35 +197,13 @@ Proof.
     apply IHM2 with (p := p) (q := q) (G := G) (l := l); try easy.
 Qed.
 
-Lemma part_step : forall pt G x6 q p l,
-    isgPartsC pt x6 ->
-    gttstepC G x6 q p l ->
-    isgPartsC pt G.
-Proof.
-  pcofix CIH. 
-  intros. 
-  induction H1 using gttstepC_ind_ref.
-  - pfold. 
-    case_eq (String.eqb pt p); intros.
-    specialize(eqb_eq pt p); intros. destruct H3. specialize(H3 H2). clear H2 H4.
-    subst. constructor.
-    case_eq (String.eqb pt q); intros.
-    specialize(eqb_eq pt q); intros. destruct H4. specialize(H4 H3). clear H3 H5. 
-    subst. constructor.
-    specialize(eqb_neq pt q); intros. destruct H4. specialize(H4 H3). clear H3 H5.
-    specialize(eqb_neq pt p); intros. destruct H3. specialize(H3 H2). clear H2 H5.
-    apply pa_send3 with (u := gc); try easy. 
-  
-
-Admitted.
-
 Lemma _3_21_ssort_helper : forall l x x2 x3,
-      Forall2
+      Forall2R
         (fun u v : option (sort * ltt) =>
          u = None \/
          (exists (s s' : sort) (t t' : ltt),
             u = Some (s, t) /\ v = Some (s', t') /\ subsort s s' /\ subtypeC t t'))
-        (extendLTT l nil (Some (x2, x3))) x ->
+        (extendLis l (Some (x2, x3))) x ->
       exists y z, onth l x = (Some (y, z)) /\ subsort x2 y.
 Proof.
   induction l; intros; try easy.
@@ -248,243 +226,22 @@ Proof.
   
 Admitted.
 
-Lemma _3_21_ssort_helper3 : forall l x x8 x0 x9,
-      Forall2
-        (fun u v : option (sort * ltt) =>
-         u = None /\ v = None \/ (exists (s : sort) (t t' : ltt), u = Some (s, t) /\ v = Some (s, t')))
-        x8 x ->
-      onth l x = Some (x0, x9) ->
-      exists x10, onth l x8 = Some(x0, x10).
-Proof.
-  induction l; intros; try easy.
-  destruct x; try easy. destruct x8; try easy. simpl in *.
-  inversion H. subst. destruct H4; try easy.
-  destruct H0. destruct H0. destruct H0. destruct H0. inversion H1. subst. exists x2. easy.
-  destruct x; try easy. destruct x8; try easy. inversion H. subst. simpl in *.
-  apply IHl with (x := x) (x9 := x9); try easy.
-Qed.
-
-Lemma _3_21_ssort_helper4 : forall l x1 x4 x5 x8 x0 x10,
-      onth l x1 = Some (x4, x5) ->
-      onth l x8 = Some (x0, x10) ->
-      Forall2
-        (fun u v : option (sort * ltt) =>
-         v = None \/
-         (exists (s s' : sort) (t t' : ltt),
-            u = Some (s, t) /\ v = Some (s', t') /\ subsort s' s /\ subtypeC t t')) x1 x8 ->
-      subsort x0 x4.
-Proof.
-  induction l; intros; try easy.
-  - destruct x1; try easy. destruct x8; try easy. simpl in *. 
-    inversion H1. subst. destruct H5; try easy.
-    destruct H. destruct H. destruct H. destruct H. destruct H. destruct H0. destruct H2. 
-    inversion H. inversion H0. subst. easy.
-  - destruct x1; try easy. destruct x8; try easy. simpl in *.
-    inversion H1. subst.
-    specialize(IHl x1 x4 x5 x8 x0 x10 H H0 H7).
-    easy.
-Qed.
-
-Lemma wfg_mon : monotone1 wfg.
-Proof.
-  unfold monotone1.
-  intros. induction IN.
-  - constructor.
-  - constructor; try easy. 
-    clear H H0. revert H1 LE. revert r r' p q.
-    induction lis; intros; try easy.
-    inversion H1. subst.
-    constructor.
-    - destruct H2. left. easy.
-    - destruct H. destruct H. destruct H. subst.
-      right. exists x. exists x0. split; try easy. apply LE. easy.
-    apply IHlis with (r := r); try easy.
-Qed.
-
-Lemma gttstep_wfc_helper : forall p q xs,
-    wfgC (gtt_send p q xs) -> 
-    List.Forall (fun u => (u = None) \/ (exists S G, u = Some(S,G) /\ wfgC G)) xs.
-Proof.
-  induction xs; intros; try easy.
-  constructor.
-  destruct a. right.
-  - destruct p0. exists s. exists g. split; try easy.
-    clear IHxs.
-    pinversion H. subst. inversion H5. subst.
-    destruct H2; try easy. destruct H0. destruct H0. destruct H0. inversion H0. subst.
-    pclearbot. easy.
-    apply wfg_mon.
-  - left. easy.
-  - pinversion H. subst.
-    specialize(SList_f a xs H4); intros. clear H4.
-    destruct H0.
-    - apply IHxs; try easy.
-      inversion H5. subst.
-      pfold. constructor; try easy.
-    - destruct H0. subst. easy.
-  - apply wfg_mon.
-Qed.
-
-Lemma gttstep_wfc_helper2 : forall xs ys,
-    SList xs ->
-    Forall2
-        (fun u v : option (sort * gtt) =>
-         u = None /\ v = None \/
-         (exists (s' : sort) (g g' : gtt), u = Some (s', g) /\ v = Some (s', g') /\ (wfgC g -> wfgC g'))) xs ys ->
-    SList ys.
-Proof.
-  induction xs; intros; try easy.
-  specialize(SList_f a xs H); intros.
-  destruct ys; try easy.
-  inversion H0. subst.
-  destruct H5.
-  - destruct H2. subst. simpl in *.
-    apply IHxs; try easy.
-  - destruct H2. destruct H2. destruct H2. destruct H2. destruct H3. subst.
-    destruct H1. 
-    apply SList_b. apply IHxs; try easy.
-    destruct H1. subst. destruct ys; try easy.
-Qed.
-
-Lemma gttstep_wfc_helper3 : forall xs ys,
-    Forall2
-        (fun u v : option (sort * gtt) =>
-         u = None /\ v = None \/
-         (exists (s' : sort) (g g' : gtt), u = Some (s', g) /\ v = Some (s', g') /\ (wfgC g -> wfgC g'))) xs ys ->
-         Forall
-        (fun u : option (sort * gtt) =>
-         u = None \/ (exists (s : sort) (t : gtt), u = Some (s, t) /\ upaco1 wfg bot1 t)) xs ->
-         Forall
-  (fun u : option (sort * gtt) =>
-   u = None \/ (exists (s0 : sort) (t : gtt), u = Some (s0, t) /\ upaco1 wfg bot1 t)) ys.
-Proof.
-  induction xs; intros; try easy.
-  destruct ys; try easy.
-  destruct ys; try easy.
-  inversion H0. subst. clear H0.
-  inversion H. subst. clear H.
-  destruct H5. 
-  - destruct H. subst. 
-    constructor. left. easy. apply IHxs; try easy.
-  - destruct H. destruct H. destruct H. destruct H. destruct H0. subst.
-    constructor. right.
-    exists x. exists x1. split; try easy.
-    destruct H3; try easy.
-    destruct H. destruct H. destruct H. inversion H. subst. clear H.
-    pclearbot.
-    specialize(H1 H0). unfold upaco1. left. easy.
-    apply IHxs; try easy.
-Qed.
-
-Lemma gttstep_wfc_helper4 : forall xs ys,
-        Forall
-        (fun u : option (sort * gtt) =>
-         u = None \/ (exists (s : sort) (t : gtt), u = Some (s, t) /\ upaco1 wfg bot1 t)) xs ->
-        Forall2
-        (fun u v : option (sort * gtt) =>
-         u = None /\ v = None \/
-         (exists (s' : sort) (g g' : gtt), u = Some (s', g) /\ v = Some (s', g') /\ (wfgC g -> wfgC g'))) xs ys ->
-        Forall
-  (fun u : option (sort * gtt) =>
-   u = None \/ (exists (s0 : sort) (t : gtt), u = Some (s0, t) /\ upaco1 wfg bot1 t)) ys.
-Proof.
-  induction xs; intros; try easy.
-  - destruct ys; try easy.
-  - destruct ys; try easy.
-    inversion H0. subst. clear H0.
-    inversion H. subst. clear H.
-    specialize(IHxs ys H3 H6).
-    constructor; try easy.
-    destruct H4. left. easy.
-    destruct H. destruct H. destruct H. destruct H. destruct H0. subst.
-    right.
-    destruct H2; try easy. destruct H. destruct H. destruct H. inversion H. subst.
-    exists x2. exists x1. split; try easy.
-    pclearbot.
-    left. apply H1; try easy.
-Qed.
 
 Lemma gttstep_wfc : forall G x8 q p l,
     wfgC G ->
     gttstepC G x8 q p l -> 
     wfgC x8.
 Proof.
-  intros. revert H. induction H0 using gttstepC_ind_ref.
-  - intros.
-    specialize(gttstep_wfc_helper p q xs H1); intros.
-    revert H0 H1 H2. revert xs. induction n; intros; try easy.
-    destruct xs; try easy.
-    - simpl in *. subst. inversion H2. subst.
-      destruct H4; try easy. destruct H0. destruct H0. destruct H0. inversion H0. subst. easy.
-    - destruct xs; try easy.
-      inversion H2. subst. simpl in *. apply IHn with (xs := xs); try easy.
-      pinversion H1. subst.
-      inversion H10. subst.
-      pfold. constructor; try easy.
-      specialize(SList_f o xs H9); intros.
-      destruct H3; try easy.
-      destruct H3. destruct H4. subst.
-      destruct n; try easy.
-    - apply wfg_mon.
-  - revert H H0 H1 H2 H3 H4 H5 H6 H7. revert p q r s ys n.
-    induction xs; intros; try easy. 
-    - pinversion H8. easy.
-      apply wfg_mon.
-    - destruct ys; try easy.
-      inversion H7. subst.
-      specialize(IHxs p q r s ys 0 H H0 H1 H2 H3 H4).
-      destruct H12. 
-      - destruct H9. subst. 
-        specialize(IHxs H5 H6 H14).
-        assert (wfgC (gtt_send r s xs)). {
-          pinversion H8. subst.
-          pfold. constructor; try easy. inversion H15. easy.
-          apply wfg_mon.
-        }
-        specialize(IHxs H9).
-        pfold. constructor; try easy.
-        - pinversion H9. subst.
-          simpl.
-          apply gttstep_wfc_helper2 with (xs := xs); try easy. 
-        apply wfg_mon.
-      - constructor. left. easy.
-        pinversion H9. subst.
-        apply gttstep_wfc_helper3 with (xs := xs); try easy.
-        apply wfg_mon.
-    - inversion H7. subst. clear H7.
-      destruct H9. destruct H7. destruct H7. destruct H7. destruct H9. subst.
-      destruct H13; try easy.
-      destruct H7. destruct H7. destruct H7. destruct H7. destruct H9.
-      inversion H7. inversion H9. subst. clear H9 H7 H17 H10.
-      simpl in *. inversion H6. subst. inversion H5. subst. clear H5 H6.
-      specialize(IHxs H15 H12 H14). 
-      pfold. constructor; try easy.
-      pinversion H8. subst.
-      specialize(SList_f (Some (x2,x3)) xs H17); intros.
-      destruct H5.
-      - apply SList_b. apply gttstep_wfc_helper2 with (xs := xs); try easy.
-      - destruct H5. subst. destruct ys; try easy.
-      apply wfg_mon.
-      constructor.
-      - right. exists x2. exists x4. split; try easy.
-        specialize(gttstep_wfc_helper r s (Some (x2,x3) :: xs) H8); intros.
-        inversion H5. subst. destruct H9; try easy.
-        destruct H6. destruct H6. destruct H6. inversion H6. subst.
-        left. apply H11; try easy.
-      pinversion H8. subst.
-      - inversion H18. subst.
-        destruct H7; try easy. destruct H5. destruct H5. destruct H5.
-        inversion H5. subst.
-        apply gttstep_wfc_helper4 with (xs := xs); try easy.
-      apply wfg_mon.
-Qed.
+    intros.
+Admitted.
 
 Theorem _3_21 : forall M M' G, typ_sess M G -> betaP M M' -> exists G', typ_sess M' G' /\ multiC G G'.
 Proof.
   intros. revert H. revert G.
   induction H0; intros; try easy.
   (* R-COMM *)
-  inversion H1. subst. rename H4 into H100. rename H5 into H4. clear H1. inversion H3. subst. clear H3.
+  inversion H1. subst. rename H4 into H100. rename H5 into H101. rename H6 into H102.
+  rename H7 into H4. clear H1. inversion H3. subst. clear H3.
   inversion H4. subst. clear H4. inversion H5. subst. clear H5.
   - inversion H4. subst. destruct H3. destruct H1. inversion H9. subst. destruct H10. destruct H5. 
   - specialize(_a23_a q xs (p_recv q xs) nil nil x H3 (eq_refl (p_recv q xs))); intros.
@@ -494,25 +251,24 @@ Proof.
   - specialize(subtype_recv x q x1 H12); intros.
     destruct H18. subst.
     specialize(subtype_recv_inv q x1 x4 H12); intros.
-    specialize(subtype_send x0 p (extendLTT l nil (Some (x2, x3))) H17); intros.
+    specialize(subtype_send x0 p (extendLis l (Some (x2, x3))) H17); intros.
     destruct H19. subst.
-    specialize(subtype_send_inv p (extendLTT l nil (Some (x2, x3))) x H17); intros.
+    specialize(subtype_send_inv p (extendLis l (Some (x2, x3))) x H17); intros.
     specialize(_3_21_ssort_helper l x x2 x3 H19); intros.
     destruct H20. destruct H20. destruct H20.
   specialize(onth_follow l xs y x1 H H13); intros. destruct H22. destruct H22.
   specialize(_3_19_h q p l G x x4 x2 x3 x1 (x6, x7) H5 H17 H1 H22 H12); intros. 
   destruct H23. exists x8.
   split.
-  constructor. 
-  - intros. unfold InT. simpl.
-    unfold InT in H2. simpl in H2. 
-    apply H2; try easy.
-    apply part_step with (x6 := x8) (q := q) (p := p) (l := l); try easy.
+  specialize(wfgC_after_step G x8 q p l H23); intros. unfold wfgC in H24. (* flagged pf *)
+  destruct H24 as [G' H105].
+  apply t_sess with (Gl := G'); intros; try easy. 
+  - apply H2; try easy. 
+    admit.
   - simpl in *. constructor. simpl.
     apply Classical_Prop.and_not_or.
     specialize(Classical_Prop.not_or_and (q = p) (In p (flattenT M)) H6); intros. destruct H20.
     split; try easy. easy.
-  apply gttstep_wfc with (G := G) (p := p) (q := q) (l := l); try easy.
   constructor. constructor. constructor.
   - specialize(_3_19_2 q p l G x8); intros.
     specialize(projection_cont_p G x8 p q l x4 H23 H1); intros.
@@ -531,10 +287,7 @@ Proof.
     assert(subsort x2 x6). { 
       apply sstrans with (s2 := x0); try easy.
       specialize(_3_21_ssort_helper2 G p q x x4 H1 H5); intros.
-      specialize(_3_21_ssort_helper3 l x x4 x0 x5 H26 H20); intros.
-      destruct H27.
-      specialize(_3_21_ssort_helper4 l x1 x6 x7 x4 x0 x10); intros.
-      apply H28; try easy.
+      admit.
     }
     apply sc_sub with (s := x2); try easy.
     apply expr_typ_multi with (e := e); try easy.
@@ -558,13 +311,13 @@ Proof.
   apply multiC_step with (G2 := x8) (p := q) (q := p) (n := l). easy. apply multiC_refl.
   
   (* T-COND *)
-  inversion H0. subst. rename H3 into H100. rename H4 into H3. 
+  inversion H0. subst. rename H3 into H100. rename H4 into H101. rename H5 into H102. rename H6 into H3. 
   inversion H3. subst. clear H3.
   inversion H6. subst. clear H6. destruct H4. destruct H3. 
   specialize(_a23_c (p_ite e P Q) e P Q x nil nil H4 (eq_refl (p_ite e P Q))); intros.
   destruct H5. destruct H5. destruct H5. destruct H6. destruct H8. destruct H9. 
   exists G. split.
-  apply t_sess; try easy. apply ForallT_par; try easy.
+  apply t_sess with (Gl := Gl); try easy. apply ForallT_par; try easy.
   apply ForallT_mono; try easy. exists x.
   split; try easy.
   apply tc_sub with (t := x0); try easy.
@@ -572,13 +325,13 @@ Proof.
   apply multiC_refl.
   
   (* F-COND *)
-  inversion H0. subst. rename H3 into H100. rename H4 into H3. 
+  inversion H0. subst. rename H3 into H100. rename H4 into H101. rename H5 into H102. rename H6 into H3. 
   inversion H3. subst. clear H3.
   inversion H6. subst. clear H6. destruct H4. destruct H3. 
   specialize(_a23_c (p_ite e P Q) e P Q x nil nil H4 (eq_refl (p_ite e P Q))); intros.
   destruct H5. destruct H5. destruct H5. destruct H6. destruct H8. destruct H9. 
   exists G. split.
-  apply t_sess; try easy. apply ForallT_par; try easy.
+  apply t_sess with (Gl := Gl); try easy. apply ForallT_par; try easy.
   apply ForallT_mono; try easy. exists x.
   split; try easy.
   apply tc_sub with (t := x1); try easy.
@@ -591,4 +344,4 @@ Proof.
   destruct H4. split; try easy.
   specialize(_a22_2 M2' M2 x H4 H0); intros. easy.
   
-Qed.
+Admitted.
