src/expressions.v
@@ -1,5 +1,6 @@
+From SST Require Import src.header. 
 Require Import List String ZArith.
-From SST Require Import src.unscoped.
+Notation fin := nat.
 
 Variant value: Type :=
   | vint : Z    -> value
@@ -24,63 +25,6 @@ Proof. intros.
        inversion H0. subst. constructor.
        easy.
 Qed.
-
-Inductive nsubsort: sort -> sort -> Prop :=
-  | nsin: nsubsort sint snat
-  | nsbi: nsubsort sbool sint
-  | nsib: nsubsort sint sbool
-  | nsbn: nsubsort sbool snat
-  | nsnb: nsubsort snat sbool
-  | nsun: nsubsort sunit snat
-  | nsnu: nsubsort snat sunit
-  | nsbu: nsubsort sbool sunit
-  | nsub: nsubsort sunit sbool
-  | nsui: nsubsort sunit sint
-  | nsiu: nsubsort sint sunit.
-
-Lemma sort_dec: forall s s', subsort s s' \/ nsubsort s s'.
-Proof. intro s.
-       induction s; intros.
-       case_eq s'; intros.
-       left. apply srefl.
-       right. apply nsub.
-       right. apply nsui.
-       right. apply nsun.
-       case_eq s'; intros.
-       right. apply nsbu.
-       left. apply srefl.
-       right. apply nsbi.
-       right. apply nsbn.
-       case_eq s'; intros.
-       right. apply nsiu.
-       right. apply nsib.
-       left. apply srefl.
-       right. apply nsin.
-       case_eq s'; intros.
-       right. apply nsnu.
-       right. apply nsnb.
-       left. apply sni.
-       left. apply srefl.
-Qed.
-
-Lemma ssnssL: forall s t, subsort s t -> (nsubsort s t -> False).
-Proof. intro s.
-       induction s; intros; case_eq t; intros; subst; try easy.
-Qed.
-
-Lemma ssnssR: forall s t, nsubsort s t -> (subsort s t -> False).
-Proof. intro s.
-       induction s; intros; case_eq t; intros; subst; try easy.
-Qed.
-
-Definition sort_eq (gs1 gs2: sort): bool :=
-  match pair gs1 gs2 with
-    | pair sint sint   => true
-    | pair sbool sbool => true
-    | pair sunit sunit => true
-    | pair snat snat   => true
-    | _                => false 
-  end.
 
 Section expr.
 Inductive expr  : Type :=
