src/header.v
@@ -1,0 +1,64 @@
+From mathcomp Require Import ssreflect.seq all_ssreflect.
+Require Import List String Coq.Arith.PeanoNat Relations.
+Import ListNotations. 
+
+Notation fin := nat.
+
+Fixpoint SList {A} (lis : list (option A)) : Prop := 
+  match lis with 
+    | Datatypes.Some x :: [] => True 
+    | _ :: xs                => SList xs
+    | []                     => False
+  end.
+
+Lemma SList_f {A} : forall x (xs : list (option A)), SList (x :: xs) -> SList xs \/ (xs = nil /\ exists a, x = Datatypes.Some a).
+Proof.
+  intros. unfold SList in H.
+  destruct x. destruct xs. right. split. easy. exists a. easy. left. easy.
+  left. easy.
+Qed.
+
+Lemma SList_b {A} : forall x (xs : list (option A)), SList xs -> SList (x :: xs).
+Proof.
+  intros. unfold SList.
+  destruct x. destruct xs; try easy. easy.
+Qed.
+
+Fixpoint extendLis {A} (n : fin) (ST : option A) : list (option A) :=
+  match n with 
+    | S m  => None :: extendLis m ST
+    | 0    => [ST]
+  end.
+
+Definition Forall2_mono {X Y} {R T : X -> Y -> Prop} (HRT : forall x y, R x y -> T x y) :
+      forall l m, Forall2 R l m -> Forall2 T l m :=
+  fix loop l m h {struct h} :=
+    match h with
+    | Forall2_nil => Forall2_nil T
+    | Forall2_cons _ _ _ _ h1 h2 => Forall2_cons _ _ (HRT _ _ h1) (loop _ _ h2)
+    end.
+
+Inductive Forall2R {X Y} (P : X -> Y -> Prop) : list X -> list Y -> Prop := 
+  | Forall2R_nil : forall ys, Forall2R P nil ys
+  | Forall2R_cons : forall x xs y ys, P x y -> Forall2R P xs ys -> Forall2R P (x :: xs) (y :: ys).
+
+Inductive multiS {X : Type} (R : relation X) : relation X :=
+  | multi_sing : forall (x y : X), R x y -> multiS R x y
+  | multi_step : forall (x y z : X), R x y -> multiS R y z -> multiS R x z.
+  
+Fixpoint onth {A : Type} (n : fin) (lis : list (option A)) : option A :=
+  match n with 
+    | S m => 
+      match lis with 
+        | x::xs => onth m xs
+        | []    => None 
+      end
+    | 0   =>
+      match lis with 
+        | x::xs => x 
+        | []    => None
+      end
+  end.
+  
+  
+  
