type/isomorphism.v
@@ -1,0 +1,57 @@
+From mathcomp Require Import ssreflect.seq all_ssreflect.
+From Paco Require Import paco pacotac.
+From SST Require Export src.expressions src.header type.global type.local.
+Require Import List String Coq.Arith.PeanoNat Relations. 
+Import ListNotations. 
+
+Inductive gnode : Type := 
+  | gnode_end : gnode
+  | gnode_pq : part -> part -> gnode
+  | gnode_s  : sort -> gnode.
+
+Inductive gttmap : global -> list fin -> option fin -> gnode -> Prop := 
+  | gmap_end : gttmap g_end nil None gnode_end
+  | gmap_pq  : forall p q xs, gttmap (g_send p q xs) nil None (gnode_pq p q)
+  | gmap_con : forall n lis xs p q st gk s gn, onth n xs = Some (st, gk) -> gttmap gk lis s gn -> gttmap (g_send p q xs) (n :: lis) s gn
+  | gmap_st  : forall n xs p q st gk, onth n xs = Some (st, gk) -> gttmap (g_send p q xs) nil (Some n) (gnode_s st)
+  | gmap_mu  : forall lis g Q s gn, subst_global 0 0 (g_rec g) g Q -> gttmap (g_rec g) lis s gn -> gttmap Q lis s gn. 
+
+
+(* global trees with context holes *)
+Inductive gtth: Type :=
+  | gtth_hol    : fin -> gtth
+  | gtth_send   : part -> part -> list (option (sort * gtth)) -> gtth.
+
+Section gtth_ind_ref.
+  Variable P : gtth -> Prop.
+  Hypothesis P_hol : forall n, P (gtth_hol n).
+  Hypothesis P_send : forall p q xs, List.Forall (fun u => u = None \/ (exists s g, u = Some(s, g) /\ P g)) xs -> P (gtth_send p q xs).
+  
+  Fixpoint gtth_ind_ref p : P p.
+  Proof.
+    destruct p.
+    - apply P_hol.
+    - apply P_send.
+      induction l; intros; try easy.
+      constructor; try easy.
+      destruct a. 
+      - destruct p. right. exists s1. exists g. split. easy. apply gtth_ind_ref.
+      - left. easy.
+  Qed.
+
+End gtth_ind_ref.
+
+Definition balancedG (G : global) := forall G w w' p q gn,
+  gttmap G w None gn -> gttmap G (w ++ w') None (gnode_pq p q) -> 
+  (exists k, forall w', gttmap G (w ++ w') None (gnode_end) \/ 
+                        (List.length w' = k /\ exists w2 w0, w' = w2 ++ w0 /\ exists r, 
+                        gttmap G (w ++ w2) None (gnode_pq p r) \/ gttmap G (w ++ w2) None (gnode_pq r p))) /\
+  (exists k, forall w', gttmap G (w ++ w') None (gnode_end) \/
+                        (List.length w' = k /\ exists w2 w0, w' = w2 ++ w0 /\ exists r,
+                        gttmap G (w ++ w2) None (gnode_pq q r) \/ gttmap G (w ++ w2) None (gnode_pq r q))).
+
+Definition wfgT G := wfG G /\ (forall n, exists m, guardG n m G) /\ balancedG G.
+
+Definition wfgC G := exists G', gttTC G' G /\ wfG G' /\ (forall n, exists m, guardG n m G') /\ balancedG G'. 
+
+Definition wfC T := exists T', lttTC T' T /\ wfL T' /\ (forall n, exists m, guardL n m T').
