type/projection.v
@@ -1,0 +1,87 @@
+From mathcomp Require Import ssreflect.seq all_ssreflect.
+From Paco Require Import paco pacotac.
+From SST Require Export src.expressions src.header type.global type.local type.isomorphism.
+Require Import List String Coq.Arith.PeanoNat Relations. 
+Import ListNotations. 
+
+Inductive isgParts : part -> global -> Prop := 
+  | pa_sendp : forall p q l, isgParts p (g_send p q l)
+  | pa_sendq : forall p q l, isgParts q (g_send p q l)
+  | pa_mu    : forall p g,   isgParts p g -> isgParts p (g_rec g)
+  | pa_sendr : forall p q r n s g lis, p <> r -> q <> r -> onth n lis = Some (s, g) -> isgParts r g -> isgParts r (g_send p q lis).
+  
+Definition isgPartsC (pt : part) (G : gtt) : Prop := 
+    exists G', gttTC G' G /\ isgParts pt G'.
+
+Fixpoint isMerge (t : ltt) (lis : list (option ltt)) : Prop := 
+  match lis with 
+    | Some x :: xs => t = x /\ isMerge t xs
+    | None   :: xs => isMerge t xs
+    | []    => True 
+  end.
+
+Variant projection (R: gtt -> part -> ltt -> Prop): gtt -> part -> ltt -> Prop :=
+  | proj_end : forall g r, 
+               wfgC g -> 
+               (isgPartsC r g -> False) -> 
+               projection R g r (ltt_end)
+  | proj_in  : forall p r xs ys,
+               wfgC (gtt_send p r xs) -> wfC (ltt_recv p ys) ->
+               List.Forall2 (fun u v => (u = None /\ v = None) \/ (exists s g t, u = Some(s, g) /\ v = Some(s, t) /\ R g r t)) xs ys ->
+               projection R (gtt_send p r xs) r (ltt_recv p ys)
+  | proj_out : forall r q xs ys,
+               wfgC (gtt_send r q xs) -> wfC (ltt_recv q ys) ->
+               List.Forall2 (fun u v => (u = None /\ v = None) \/ (exists s g t, u = Some(s, g) /\ v = Some(s, t) /\ R g r t)) xs ys ->
+               projection R (gtt_send r q xs) r (ltt_send q ys)
+  | proj_cont: forall p q r xs ys t,
+               wfgC (gtt_send p q xs) -> wfC t ->
+               q <> r ->
+               p <> r ->
+               t <> ltt_end ->
+               List.Forall2 (fun u v => (u = None /\ v = None) \/ (exists s g t, u = Some(s, g) /\ v = Some t /\ R g r t)) xs ys ->
+               isMerge t ys ->
+               projection R (gtt_send p q xs) r t.
+
+Definition projectionC g r t := paco3 projection bot3 g r t.
+
+Lemma proj_mon: monotone3 projection.
+Proof. unfold monotone3.
+       intros.
+       induction IN; intros.
+       - constructor. easy.
+       - try easy.
+Admitted.
+
+Lemma pmergeCR: forall G r,
+          projectionC G r ltt_end ->
+          (isgPartsC r G -> False).
+Proof. intros.
+       pinversion H. subst. apply H2. easy. subst. easy.
+       apply proj_mon.
+Qed.
+
+Variant gttstep (R: gtt -> gtt -> part -> part -> nat -> Prop): gtt -> gtt -> part -> part -> nat -> Prop :=
+  | steq : forall p q xs s gc n,
+                  wfgC (gtt_send p q xs) -> 
+                  p <> q ->
+                  Datatypes.Some (s, gc) = onth n xs ->
+                  gttstep R (gtt_send p q xs) gc p q n
+  | stneq: forall p q r s xs ys n,
+                  wfgC (gtt_send p q xs) ->
+                  p <> q ->
+                  r <> s ->
+                  r <> p ->
+                  r <> q ->
+                  s <> p ->
+                  s <> q ->
+                  List.Forall (fun u => u = None \/ (exists s g, u = Some(s, g) /\ isgPartsC p g /\ isgPartsC q g)) xs ->
+                  List.Forall2 (fun u v => (u = None /\ v = None) \/ (exists s g g', u = Some(s, g) /\ v = Some(s, g') /\ R g g' p q n)) xs ys ->
+                  gttstep R (gtt_send r s xs) (gtt_send r s ys) p q n.
+
+Definition gttstepC g1 g2 p q n := paco5 gttstep bot5 g1 g2 p q n. 
+
+Lemma wfgC_after_step : forall G G' p q n, gttstepC G G' p q n -> wfgC G'.
+Proof.
+Admitted.
+
+
